thys/lib/More_Refine_Util.thy
@@ -4,21 +4,21 @@ begin
 
   ML \<open>
   
-    signature REFINE_UTIL = sig
+    signature MORE_REFINE_UTIL = sig
       include REFINE_UTIL
       
       
       (* Prove premises of theorem by given tactics. Warning: Simultaneous semantics, 
         will fail/misbehave if tactic instantiates schematic that occurs in later premise to be proved *)
-      val prove_prems: Proof.context -> thm -> (Proof.context -> int -> tactic) option list -> thm
+      val prove_prems: bool -> Proof.context -> thm -> (Proof.context -> int -> tactic) option list -> thm
       
     end
   
     
-    structure Refine_Util : REFINE_UTIL = struct
+    structure More_Refine_Util : MORE_REFINE_UTIL = struct
       open Refine_Util
   
-      fun prove_prems ctxt thm tacs = let
+      fun prove_prems tryflag ctxt thm tacs = let
         
         fun mk_cnv [] = Conv.all_conv
           | mk_cnv (NONE::xs) = Conv.implies_concl_conv (mk_cnv xs)
@@ -27,17 +27,24 @@ begin
         (* Atomize relevant premises *)  
         val thm = Conv.fconv_rule (mk_cnv tacs) thm
           
+
         fun prove t tac = Goal.prove ctxt [] [] t (fn {context=ctxt, ...} => 
           ALLGOALS (
             REPEAT_DETERM' (match_tac ctxt @{thms allI impI}) (* TODO: Maybe apply atomize-rules in reverse *)
             THEN' tac ctxt
           ) 
         )
+
+        fun try_prove t tac =
+          case (try (prove t) tac ) of SOME thm => thm
+              | NONE => asm_rl
         
+        val prove_t = (if tryflag then try_prove else prove)
+
         fun proves [] _ = []
           | proves _ [] = []
           | proves (_::ps) (NONE::tacs) = asm_rl :: proves ps tacs
-          | proves (p::ps) (SOME tac :: tacs) = prove p tac :: proves ps tacs
+          | proves (p::ps) (SOME tac :: tacs) = prove_t p tac :: proves ps tacs
           
         (* Prove premises *)  
         val pthms = proves (Thm.prems_of thm) tacs
